theories/base_logic/lib/wsat.v
@@ -1,46 +1,99 @@
 From stdpp Require Export coPset.
 From iris.proofmode Require Import tactics.
-From iris.algebra Require Import gmap auth agree gset coPset.
+From iris.algebra Require Import gmap auth agree gset coPset list vector excl mlist.
 From iris.base_logic.lib Require Export own.
 Set Default Proof Using "Type".
+
+(* An inductive grammar of "basic" BI expressions. *)
+Inductive bi_schema :=
+| bi_sch_emp : bi_schema
+| bi_sch_pure : Prop → bi_schema
+| bi_sch_and : bi_schema → bi_schema → bi_schema
+| bi_sch_or : bi_schema → bi_schema → bi_schema
+| bi_sch_forall : ∀ A, (A → bi_schema) → bi_schema
+| bi_sch_exist : ∀ A, (A → bi_schema) → bi_schema
+| bi_sch_sep : bi_schema → bi_schema → bi_schema
+| bi_sch_wand : bi_schema → bi_schema → bi_schema
+| bi_sch_persistently : bi_schema → bi_schema
+| bi_sch_later : bi_schema → bi_schema
+| bi_sch_bupd : bi_schema → bi_schema
+(* Schemas can include either fixed or mutable references to an iProp *)
+| bi_sch_var_fixed : nat → bi_schema
+| bi_sch_var_mut : nat → bi_schema
+| bi_sch_wsat : bi_schema
+| bi_sch_ownE : coPset → bi_schema.
+
+Canonical Structure bi_schemaO := leibnizO bi_schema.
 
 (** All definitions in this file are internal to [fancy_updates] with the
 exception of what's in the [invG] module. The module [invG] is thus exported in
 [fancy_updates], which [wsat] is only imported. *)
+
+Record invariant_level_names := { invariant_name : gname; }.
+
+Global Instance invariant_level_names_eq_dec : EqDecision (invariant_level_names).
+Proof.
+  intros [] [].
+  rewrite /Decision.
+  repeat (decide equality).
+Qed.
+
 Module invG.
   Class invG (Σ : gFunctors) : Set := WsatG {
-    inv_inG :> inG Σ (authR (gmapUR positive (agreeR (laterO (iPrePropO Σ)))));
+    inv_inG :> inG Σ (authR (gmapUR positive
+                                    (prodR (agreeR (prodO (listO (laterO (iPrePropO Σ))) bi_schemaO))
+                                           (optionUR (prodR fracR (agreeR (listO (laterO (iPrePropO Σ)))))))));
     enabled_inG :> inG Σ coPset_disjR;
     disabled_inG :> inG Σ (gset_disjR positive);
-    invariant_name : gname;
+    mlist_inG :> fmlistG (invariant_level_names) Σ;
+    inv_list_name : gname;
     enabled_name : gname;
     disabled_name : gname;
   }.
 
   Definition invΣ : gFunctors :=
-    #[GFunctor (authRF (gmapURF positive (agreeRF (laterOF idOF))));
+    #[GFunctor (authRF (gmapURF positive
+                                (prodRF (agreeRF (prodOF (listOF (laterOF idOF)) (constOF bi_schemaO)))
+                                        (optionRF (prodRF fracR (agreeRF (listOF (laterOF idOF))))))));
       GFunctor coPset_disjUR;
-      GFunctor (gset_disjUR positive)].
+      GFunctor (gset_disjUR positive);
+      fmlistΣ invariant_level_names
+     ].
 
   Class invPreG (Σ : gFunctors) : Set := WsatPreG {
-    inv_inPreG :> inG Σ (authR (gmapUR positive (agreeR (laterO (iPrePropO Σ)))));
+    inv_inPreG :> inG Σ (authR (gmapUR positive
+                                    (prodR (agreeR (prodO (listO (laterO (iPrePropO Σ))) bi_schemaO))
+                                           (optionUR (prodR fracR (agreeR (listO (laterO (iPrePropO Σ)))))))));
     enabled_inPreG :> inG Σ coPset_disjR;
     disabled_inPreG :> inG Σ (gset_disjR positive);
+    mlist_inPreG :> fmlistG (invariant_level_names) Σ;
   }.
 
+  (* XXX: this is very slow for some reason. *)
   Instance subG_invΣ {Σ} : subG invΣ Σ → invPreG Σ.
   Proof. solve_inG. Qed.
 End invG.
 Import invG.
 
-Definition invariant_unfold {Σ} (P : iProp Σ) : agree (later (iPrePropO Σ)) :=
-  to_agree (Next (iProp_unfold P)).
-Definition ownI `{!invG Σ} (i : positive) (P : iProp Σ) : iProp Σ :=
-  own invariant_name (◯ {[ i := invariant_unfold P ]}).
-Arguments ownI {_ _} _ _%I.
+Definition invariant_unfold {Σ} {n} sch (Ps : vec (iProp Σ) n) : agree (list (later (iPrePropO Σ)) * bi_schema) :=
+  to_agree ((λ P, Next (iProp_unfold P)) <$> (vec_to_list Ps), sch).
+Definition inv_mut_unfold {Σ} {n} q (Ps : vec (iProp Σ) n) : option (frac * (agree (list (later (iPrePropO Σ))))) :=
+  Some (q%Qp, to_agree ((λ P, Next (iProp_unfold P)) <$> (vec_to_list Ps))).
+Definition ownI `{!invG Σ} {n} (lvl: nat) (i : positive) (sch: bi_schema) (Ps : vec (iProp Σ) n) : iProp Σ :=
+  (∃ γs, fmlist_idx inv_list_name lvl γs ∗
+         own (invariant_name γs) (◯ {[ i := (invariant_unfold sch Ps, ε) ]})).
+Arguments ownI {_ _ _} _ _ _%I _%I.
 Typeclasses Opaque ownI.
 Instance: Params (@invariant_unfold) 1 := {}.
 Instance: Params (@ownI) 3 := {}.
+
+Definition ownI_mut `{!invG Σ} {n} (lvl: nat) (i : positive) q (Qs : vec (iProp Σ) n) : iProp Σ :=
+  (∃ (l: agree (list (later (iPrePropO Σ)) * bi_schema)) γs, fmlist_idx inv_list_name lvl γs ∗
+         own (invariant_name γs) (◯ {[ i := (l, inv_mut_unfold q Qs) ]})).
+Arguments ownI_mut {_ _ _} _ _ _%I.
+Typeclasses Opaque ownI_mut.
+Instance: Params (@inv_mut_unfold) 1 := {}.
+Instance: Params (@ownI_mut) 3 := {}.
 
 Definition ownE `{!invG Σ} (E : coPset) : iProp Σ :=
   own enabled_name (CoPset E).
@@ -52,21 +105,160 @@ Definition ownD `{!invG Σ} (E : gset positive) : iProp Σ :=
 Typeclasses Opaque ownD.
 Instance: Params (@ownD) 3 := {}.
 
-Definition wsat `{!invG Σ} : iProp Σ :=
-  locked (∃ I : gmap positive (iProp Σ),
-    own invariant_name (● (invariant_unfold <$> I : gmap _ _)) ∗
-    [∗ map] i ↦ Q ∈ I, ▷ Q ∗ ownD {[i]} ∨ ownE {[i]})%I.
+Definition inv_cmra_fmap `{!invG Σ} (v: (list (iProp Σ) * bi_schema) * list (iProp Σ)) :=
+  let '((Ps, sch), Qs) := v in
+  (invariant_unfold sch (list_to_vec Ps), inv_mut_unfold 1%Qp (list_to_vec Qs)).
+
+Fixpoint bi_schema_pre `{!invG Σ} (Ps Ps_mut: list (iProp Σ)) wsat (sch: bi_schema) :=
+  match sch with
+  | bi_sch_emp => emp
+  | bi_sch_pure φ => ⌜φ⌝
+  | bi_sch_and sch1 sch2 => bi_schema_pre Ps Ps_mut wsat sch1 ∧ bi_schema_pre Ps Ps_mut wsat sch2
+  | bi_sch_or sch1 sch2 => bi_schema_pre Ps Ps_mut wsat sch1 ∨ bi_schema_pre Ps Ps_mut wsat sch2
+  | bi_sch_forall A sch => ∀ (a: A),  bi_schema_pre Ps Ps_mut wsat (sch a)
+  | bi_sch_exist A sch => ∃ (a: A),  bi_schema_pre Ps Ps_mut wsat (sch a)
+  | bi_sch_sep sch1 sch2 => bi_schema_pre Ps Ps_mut wsat sch1 ∗ bi_schema_pre Ps Ps_mut wsat sch2
+  | bi_sch_wand sch1 sch2 => bi_schema_pre Ps Ps_mut wsat sch1 -∗ bi_schema_pre Ps Ps_mut wsat sch2
+  | bi_sch_persistently sch => <pers> bi_schema_pre Ps Ps_mut wsat sch
+  | bi_sch_later sch => ▷ bi_schema_pre Ps Ps_mut wsat sch
+  | bi_sch_bupd sch => |==> bi_schema_pre Ps Ps_mut wsat sch
+  | bi_sch_var_fixed i =>
+    match (Ps !! i) with
+    | None => emp
+    | Some P => P
+    end
+  | bi_sch_var_mut i =>
+    match (Ps_mut !! i) with
+    | None => emp
+    | Some P => P
+    end
+  | bi_sch_wsat => wsat
+  | bi_sch_ownE E => ownE E
+  end%I.
+
+Definition wsat_pre `{!invG Σ} n bi_schema_interp :=
+  (∃ I : gmap positive ((list (iProp Σ) * bi_schema) * list (iProp Σ)),
+        (∃ γs, fmlist_idx inv_list_name n γs ∗
+             own (invariant_name γs) (● (inv_cmra_fmap <$> I : gmap _ _))) ∗
+        [∗ map] i ↦ Qs ∈ I, (bi_schema_interp (bi_later <$> Qs.1.1) (bi_later <$> Qs.2) Qs.1.2 ∗
+                             ownI_mut n i (1/2)%Qp (list_to_vec Qs.2) ∗
+                             ownD {[i]}) ∨
+                            ownE {[i]})%I.
+
+Fixpoint bi_schema_interp `{!invG Σ} n (Ps Ps_mut: list (iProp Σ)) sch {struct n} :=
+  match n with
+  | O => bi_schema_pre Ps Ps_mut True%I sch
+  | S n' => bi_schema_pre Ps Ps_mut (wsat_pre n' (bi_schema_interp n') ∗ wsat n')%I sch
+  end
+  with
+  wsat `{!invG Σ} n :=
+  match n with
+    | S n =>
+  (∃ I : gmap positive ((list (iProp Σ) * bi_schema) * list (iProp Σ)),
+        (∃ γs, fmlist_idx inv_list_name n γs ∗
+             own (invariant_name γs) (● (inv_cmra_fmap <$> I : gmap _ _))) ∗
+        [∗ map] i ↦ Qs ∈ I, (bi_schema_interp n (bi_later <$> Qs.1.1) (bi_later <$> Qs.2) Qs.1.2 ∗
+                             ownI_mut n i (1/2)%Qp (list_to_vec Qs.2) ∗
+                             ownD {[i]}) ∨
+                            ownE {[i]})
+    ∗ wsat n
+    | O => True
+  end%I.
+Arguments bi_schema_interp {_ _} _ _ _ _.
+Arguments wsat {_ _} _.
+
+Lemma wsat_unfold `{!invG Σ} n:
+  wsat n =
+  match n with
+    | S n =>
+  (∃ I : gmap positive ((list (iProp Σ) * bi_schema) * list (iProp Σ)),
+        (∃ γs, fmlist_idx inv_list_name n γs ∗
+             own (invariant_name γs) (● (inv_cmra_fmap <$> I : gmap _ _))) ∗
+        [∗ map] i ↦ Qs ∈ I, (bi_schema_interp n (bi_later <$> Qs.1.1) (bi_later <$> Qs.2) Qs.1.2 ∗
+                             ownI_mut n i (1/2)%Qp (list_to_vec Qs.2) ∗
+                             ownD {[i]}) ∨
+                            ownE {[i]})
+    ∗ wsat n
+    | O => True
+  end%I.
+Proof. rewrite /=. destruct n => //=. Qed.
+
+Lemma bi_schema_interp_unfold `{!invG Σ} n Ps Ps_mut sch :
+  bi_schema_interp n Ps Ps_mut sch =
+  match sch with
+  | bi_sch_emp => emp
+  | bi_sch_pure φ => ⌜φ⌝
+  | bi_sch_and sch1 sch2 => bi_schema_interp n Ps Ps_mut sch1 ∧ bi_schema_interp n Ps Ps_mut sch2
+  | bi_sch_or sch1 sch2 => bi_schema_interp n Ps Ps_mut sch1 ∨ bi_schema_interp n Ps Ps_mut sch2
+  | bi_sch_forall A sch => ∀ (a: A),  bi_schema_interp n Ps Ps_mut (sch a)
+  | bi_sch_exist A sch => ∃ (a: A),  bi_schema_interp n Ps Ps_mut (sch a)
+  | bi_sch_sep sch1 sch2 => bi_schema_interp n Ps Ps_mut sch1 ∗ bi_schema_interp n Ps Ps_mut sch2
+  | bi_sch_wand sch1 sch2 => bi_schema_interp n Ps Ps_mut sch1 -∗ bi_schema_interp n Ps Ps_mut sch2
+  | bi_sch_persistently sch => <pers> bi_schema_interp n Ps Ps_mut sch
+  | bi_sch_later sch => ▷ bi_schema_interp n Ps Ps_mut sch
+  | bi_sch_bupd sch => |==> bi_schema_interp n Ps Ps_mut sch
+  | bi_sch_var_fixed i =>
+    match (Ps !! i) with
+    | None => emp
+    | Some P => P
+    end
+  | bi_sch_var_mut i =>
+    match (Ps_mut !! i) with
+    | None => emp
+    | Some P => P
+    end
+  | bi_sch_wsat => wsat n
+  | bi_sch_ownE E => ownE E
+  end%I.
+Proof. destruct n, sch => //=. Qed.
+
+Opaque wsat bi_schema_interp_unfold.
 
 Section wsat.
 Context `{!invG Σ}.
 Implicit Types P : iProp Σ.
 
+Lemma wsat_le_acc n1 n2:
+  n1 ≤ n2 →
+  wsat n2 ⊢ wsat n1 ∗ (wsat n1 -∗ wsat n2).
+Proof.
+  induction 1.
+  - iIntros "$". eauto.
+  - rewrite wsat_unfold.
+    iIntros "($&Hm)".
+    iDestruct (IHle with "Hm") as "($&Hclo)".
+    auto.
+Qed.
+
 (* Invariants *)
-Instance invariant_unfold_contractive : Contractive (@invariant_unfold Σ).
-Proof. solve_contractive. Qed.
-Global Instance ownI_contractive i : Contractive (@ownI Σ _ i).
-Proof. solve_contractive. Qed.
-Global Instance ownI_persistent i P : Persistent (ownI i P).
+Lemma dist_later_vec_to_list {A: ofeT} {m} n (l1 l2 : vec A m):
+  dist_later n l1 l2 ↔ dist_later n (vec_to_list l1) (vec_to_list l2).
+Proof. destruct n => //=. Qed.
+Instance invariant_unfold_contractive' m sch : Contractive (@invariant_unfold Σ m sch).
+Proof.
+  intros n l1 l2 Hd.
+  rewrite /invariant_unfold.
+  specialize (vec_to_list_same_length l1 l2) => Hlen.
+  rewrite dist_later_vec_to_list in Hd *.
+  remember (vec_to_list l1) as l1' eqn:Heq1.
+  remember (vec_to_list l2) as l2' eqn:Heq2.
+  rewrite -Heq1 -Heq2.
+  clear l1 l2 Heq1 Heq2.
+  revert l2' Hlen.
+  induction l1' => l2' Hlen Hd.
+  - destruct l2' => //=.
+  - destruct l2'; first by (simpl in Hlen; congruence).
+    apply to_agree_ne => //=.
+    apply pair_ne; last done. econstructor.
+    { destruct n; eauto. apply Next_contractive. inversion Hd; subst; eauto => //=.
+      by f_equiv. }
+    efeed pose proof (IHl1' l2') as Hagree; eauto.
+    { destruct n; eauto. inversion Hd; subst; eauto. }
+    apply to_agree_injN in Hagree. eapply Hagree.
+Qed.
+Global Instance ownI_contractive n lvl i sch : Contractive (@ownI Σ _ n lvl i sch).
+Proof. rewrite /ownI. solve_contractive. Qed.
+Global Instance ownI_persistent n lvl i sch (Ps: vec _ n) : Persistent (ownI lvl i sch Ps).
 Proof. rewrite /ownI. apply _. Qed.
 
 Lemma ownE_empty : ⊢ |==> ownE ∅.
@@ -105,53 +297,473 @@ Qed.
 Lemma ownD_singleton_twice i : ownD {[i]} ∗ ownD {[i]} ⊢ False.
 Proof. rewrite ownD_disjoint. iIntros (?); set_solver. Qed.
 
-Lemma invariant_lookup (I : gmap positive (iProp Σ)) i P :
-  own invariant_name (● (invariant_unfold <$> I : gmap _ _)) ∗
-  own invariant_name (◯ {[i := invariant_unfold P]}) ⊢
-  ∃ Q, ⌜I !! i = Some Q⌝ ∗ ▷ (Q ≡ P).
+Lemma list_equivI_O {A: ofeT} {M} (m1 m2: list A) : m1 ≡ m2 ⊣⊢@{uPredI M} ∀ i, m1 !! i ≡ m2 !! i.
+Proof.
+  uPred.unseal => //=.
+  split => n x Hval. split.
+  - intros ? Hequiv. apply list_dist_lookup; eauto.
+  - intros Hequiv. apply list_dist_lookup; eauto.
+Qed.
+Lemma list_equivI_1 {A: ofeT} {M} (m1 m2: list A) : m1 ≡ m2 ⊢@{uPredI M} ∀ i, m1 !! i ≡ m2 !! i.
+Proof.
+  uPred.unseal => //=.
+  split => n x Hval Hequiv i. apply list_dist_lookup; eauto.
+Qed.
+Lemma list_equivI_length {A: ofeT} {M} (m1 m2: list A) : m1 ≡ m2 ⊢@{uPredI M} ⌜ length m1 = length m2 ⌝.
+Proof.
+  uPred.unseal => //=.
+  split => n x Hval Hequiv.
+  eapply (Forall2_length _ m1 m2 Hequiv).
+Qed.
+Lemma vec_equivI_1 {A: ofeT} {M} {n} (m1 m2: vec A n) :
+  m1 ≡ m2 ⊢@{uPredI M} ∀ i, vec_to_list m1 !! i ≡ vec_to_list m2 !! i.
+Proof.
+  uPred.unseal => //=.
+  split => ? x Hval Hequiv i. apply list_dist_lookup; eauto.
+Qed.
+
+Lemma invariant_lookup_weak I {n} γ i sch (Ps: vec _ n) :
+  own γ (● (inv_cmra_fmap <$> I : gmap _ _)) ∗
+  own γ (◯ {[i := (invariant_unfold sch Ps, ε)]})  ⊢
+  ∃ Qs Qs_mut, ⌜I !! i = Some ((Qs, sch), Qs_mut)⌝ ∗
+               ⌜ length Qs = length Ps ⌝ ∗
+               ∀ i, ▷ (Qs !! i ≡ vec_to_list Ps !! i).
 Proof.
   rewrite -own_op own_valid auth_both_validI /=. iIntros "[_ [#HI #HvI]]".
   iDestruct "HI" as (I') "HI". rewrite gmap_equivI gmap_validI.
   iSpecialize ("HI" $! i). iSpecialize ("HvI" $! i).
   rewrite lookup_fmap lookup_op lookup_singleton option_equivI.
-  case: (I !! i)=> [Q|] /=; [|case: (I' !! i)=> [Q'|] /=; by iExFalso].
-  iExists Q; iSplit; first done.
-  iAssert (invariant_unfold Q ≡ invariant_unfold P)%I as "?".
-  { case: (I' !! i)=> [Q'|] //=.
-    iRewrite "HI" in "HvI". rewrite uPred.option_validI agree_validI.
-    iRewrite -"HvI" in "HI". by rewrite agree_idemp. }
+  case: (I !! i)=> [[[Q sch'] Qmut]|] /=; [|case: (I' !! i)=> [Q'|] /=; by iExFalso].
+  iExists Q, Qmut. (* iSplit; first done. *)
+  iAssert (invariant_unfold sch' (list_to_vec Q) ≡ invariant_unfold sch Ps)%I as "Hequiv".
+  { case: (I' !! i)=> [[Q' Qmut']|] //=.
+    - iRewrite "HI" in "HvI". rewrite uPred.option_validI uPred.prod_validI agree_validI.
+      iDestruct "HvI" as "(HvI&_)". simpl.
+      iRewrite -"HvI" in "HI". rewrite -pair_op agree_idemp prod_equivI.
+      iDestruct "HI" as "($&_)".
+    - rewrite prod_equivI. iDestruct "HI" as "($&_)".
+  }
   rewrite /invariant_unfold.
-  by rewrite agree_equivI later_equivI iProp_unfold_equivI.
+  rewrite agree_equivI prod_equivI //=. iDestruct "Hequiv" as "(Hequiv&Hsch_equiv)".
+  iSplit.
+  { iDestruct "Hsch_equiv" as %Heq. iPureIntro. move:Heq => //=. congruence. }
+  iDestruct (list_equivI_length with "Hequiv") as %Hlen.
+  iSplit.
+  { iPureIntro. move: Hlen. rewrite ?fmap_length vec_to_list_to_vec //=. }
+  rewrite list_equivI_1. iIntros (j).
+  iSpecialize ("Hequiv" $! j).
+  rewrite ?list_lookup_fmap vec_to_list_to_vec.
+  rewrite option_equivI.
+  destruct (Q !! j) as [Q0|] eqn:HeqQ;
+  destruct (vec_to_list Ps !! j) as [P0|] eqn:HeqP;
+  rewrite ?HeqQ ?HeqP //=.
+  { rewrite //= ?later_equivI iProp_unfold_equivI //=. iNext. by iRewrite "Hequiv". }
 Qed.
 
-Lemma ownI_open i P : wsat ∗ ownI i P ∗ ownE {[i]} ⊢ wsat ∗ ▷ P ∗ ownD {[i]}.
+Lemma agree_equiv_inclI {M} {A: ofeT} (a b: A) c : to_agree a ≡ to_agree b ⋅ c ⊢@{uPredI M} (b ≡ a).
 Proof.
-  rewrite /ownI /wsat -!lock.
-  iIntros "(Hw & Hi & HiE)". iDestruct "Hw" as (I) "[Hw HI]".
-  iDestruct (invariant_lookup I i P with "[$]") as (Q ?) "#HPQ".
-  iDestruct (big_sepM_delete _ _ i with "HI") as "[[[HQ $]|HiE'] HI]"; eauto.
-  - iSplitR "HQ"; last by iNext; iRewrite -"HPQ".
-    iExists I. iFrame "Hw". iApply (big_sepM_delete _ _ i); eauto.
+  uPred.unseal. split.
+  intros n ? Hx Heq. apply (to_agree_includedN n b a). exists c; eauto.
+Qed.
+
+Lemma agree_op_invI {M} {A : ofeT} (x y : agree A): ✓ (x ⋅ y) ⊢@{uPredI M} x ≡ y.
+Proof. uPred.unseal. split. intros n ? Hx Heq. by apply agree_op_invN. Qed.
+
+Lemma invariant_lookup_strong I {n m} γ i q sch (Ps: vec _ n) (Ps_mut: vec _ m) :
+  own γ (● (inv_cmra_fmap <$> I : gmap _ _)) ∗
+  own γ (◯ {[i := (invariant_unfold sch Ps, inv_mut_unfold q Ps_mut)]})  ⊢
+  ∃ Qs Qs_mut, ⌜I !! i = Some ((Qs, sch), Qs_mut)⌝ ∗
+               ⌜ length Qs = length Ps ⌝ ∗
+               ⌜ length Qs_mut = length Ps_mut ⌝ ∗
+               (∀ i, ▷ (Qs !! i ≡ vec_to_list Ps !! i)) ∗
+               (∀ i, ▷ (Qs_mut !! i ≡ vec_to_list Ps_mut !! i)).
+Proof.
+  rewrite -own_op own_valid auth_both_validI /=. iIntros "[_ [#HI #HvI]]".
+  iDestruct "HI" as (I') "HI". rewrite gmap_equivI gmap_validI.
+  iSpecialize ("HI" $! i). iSpecialize ("HvI" $! i).
+  rewrite lookup_fmap lookup_op lookup_singleton option_equivI.
+  case: (I !! i)=> [[[Q sch'] Qmut]|] /=; [|case: (I' !! i)=> [Q'|] /=; by iExFalso].
+  iExists Q, Qmut. (* iSplit; first done. *)
+  iAssert (invariant_unfold sch' (list_to_vec Q) ≡ invariant_unfold sch Ps)%I as "Hequiv".
+  { case: (I' !! i)=> [[Q' Qmut']|] //=.
+    - iRewrite "HI" in "HvI". rewrite uPred.option_validI uPred.prod_validI agree_validI.
+      iDestruct "HvI" as "(HvI&_)". simpl.
+      iRewrite -"HvI" in "HI". rewrite -pair_op agree_idemp prod_equivI.
+      iDestruct "HI" as "($&_)".
+    - rewrite prod_equivI. iDestruct "HI" as "($&_)".
+  }
+  (* XXX: this asserts a bundled equivalence that we then break apart right afterward. *)
+  iAssert (inv_mut_unfold q (list_to_vec Qmut) ≡ inv_mut_unfold q Ps_mut)%I as "Hequiv_mut".
+  {
+    case: (I' !! i)=> [[Q' Qmut']|] //=.
+    - iRewrite "HI" in "HvI". rewrite uPred.option_validI uPred.prod_validI agree_validI.
+      iDestruct "HvI" as "(HvI&_)". simpl.
+      iRewrite -"HvI" in "HI". rewrite -pair_op agree_idemp prod_equivI //=.
+      iDestruct "HI" as "(_&Hi)".
+      rewrite /inv_mut_unfold option_equivI ?prod_equivI; iSplit => //=.
+      destruct Qmut' as [(?&?)|]; last first.
+      { iEval (rewrite right_id) in "Hi".
+        rewrite option_equivI prod_equivI; iDestruct "Hi" as "(_&$)". }
+      rewrite -Some_op -pair_op.
+      rewrite option_equivI prod_equivI. iDestruct "Hi" as "(_&Hi)" => //=.
+      iDestruct (agree_equiv_inclI with "Hi") as "Heq". by iRewrite "Heq".
+    - rewrite prod_equivI => //=.
+      rewrite /inv_mut_unfold ?option_equivI ?prod_equivI; iSplit => //=.
+      iDestruct "HI" as "(_&_&$)".
+  }
+  rewrite /invariant_unfold.
+  rewrite agree_equivI prod_equivI //=. iDestruct "Hequiv" as "(Hequiv&Hsch_equiv)".
+  rewrite /inv_mut_unfold.
+  rewrite option_equivI prod_equivI agree_equivI. iDestruct "Hequiv_mut" as "(_&Hequiv_mut)".
+  iSplit.
+  { iDestruct "Hsch_equiv" as %Heq. iPureIntro. move:Heq => //=. congruence. }
+  iDestruct (list_equivI_length with "Hequiv") as %Hlen.
+  iDestruct (list_equivI_length with "Hequiv_mut") as %Hlen_mut.
+  iSplit.
+  { iPureIntro. move: Hlen. rewrite ?fmap_length vec_to_list_to_vec //=. }
+  iSplit.
+  { iPureIntro. move: Hlen_mut. rewrite ?fmap_length vec_to_list_to_vec //=. }
+  rewrite ?list_equivI_1.
+  iSplitL "Hequiv HI".
+  - iIntros (j).
+    iSpecialize ("Hequiv" $! j).
+    rewrite ?list_lookup_fmap ?vec_to_list_to_vec.
+    rewrite option_equivI.
+    destruct (Q !! j) as [Q0|] eqn:HeqQ;
+    destruct (vec_to_list Ps !! j) as [P0|] eqn:HeqP;
+    rewrite ?HeqQ ?HeqP //=.
+    { rewrite //= ?later_equivI iProp_unfold_equivI //=. iNext. by iRewrite "Hequiv". }
+  - iIntros (j).
+    iSpecialize ("Hequiv_mut" $! j).
+    rewrite ?list_lookup_fmap ?vec_to_list_to_vec.
+    rewrite option_equivI.
+    destruct (Qmut !! j) as [Q0|] eqn:HeqQ;
+    destruct (vec_to_list Ps_mut !! j) as [P0|] eqn:HeqP;
+    rewrite ?HeqQ ?HeqP //=.
+    { rewrite //= ?later_equivI iProp_unfold_equivI //=. iNext. by iRewrite "Hequiv_mut". }
+Qed.
+
+
+Lemma equivI_elim_own {A: cmraT} `{Hin: inG Σ A} γ (a b: A):
+  (a ≡ b) -∗ own γ a -∗ own γ b.
+Proof. iIntros "Hequiv". iRewrite "Hequiv". eauto. Qed.
+
+Lemma ownI_mut_later {n m} lvl i q (Qs_mut: vec _ n) (Ps_mut: vec _ m):
+  n = m →
+  (∀ i, ▷ (vec_to_list Qs_mut !! i ≡ vec_to_list Ps_mut !! i)) -∗
+  ownI_mut lvl i q (Qs_mut) -∗
+  ownI_mut lvl i q (Ps_mut).
+Proof.
+  iIntros (Hlen) "#HPQ". rewrite /ownI_mut.
+  iDestruct 1 as (l γs) "(Hidx&Hown)".
+  iExists l, γs; iFrame.
+  iApply (equivI_elim_own with "[] Hown").
+  { rewrite auth_equivI => //=. iSplit; first done.
+    rewrite gmap_equivI. iIntros (i0).
+    destruct (decide (i = i0)).
+    { subst. rewrite ?lookup_singleton option_equivI prod_equivI => //=.
+      iSplit; first done.
+      rewrite /inv_mut_unfold option_equivI prod_equivI => //=; iSplit; first done.
+      rewrite agree_equivI ?vec_to_list_to_vec list_equivI_O.
+      iIntros (j).
+      rewrite ?list_lookup_fmap.
+      iSpecialize ("HPQ" $! j).
+      rewrite ?option_equivI.
+      destruct (vec_to_list Qs_mut !! j) as [Q0|] eqn:HeqQ;
+      destruct (vec_to_list Ps_mut !! j) as [P0|] eqn:HeqP;
+      rewrite ?HeqQ ?HeqP //=.
+      * rewrite later_equivI. iNext. by iRewrite "HPQ".
+      * exfalso. apply lookup_ge_None_1 in HeqP. apply lookup_lt_Some in HeqQ.
+        rewrite ?vec_to_list_length in HeqQ HeqP. lia.
+      * exfalso. apply lookup_ge_None_1 in HeqQ. apply lookup_lt_Some in HeqP.
+        rewrite ?vec_to_list_length in HeqQ HeqP. lia.
+    }
+    rewrite ?lookup_singleton_ne //=.
+  }
+Qed.
+
+Lemma bi_schema_interp_ctx_later lvl sch (Qs Qs_mut Ps Ps_mut: list (iProp Σ)):
+  (∀ i, ▷ (Qs !! i ≡ Ps !! i)) -∗
+  (∀ i, ▷ (Qs_mut !! i ≡ Ps_mut !! i)) -∗
+  bi_schema_interp lvl (bi_later <$> Qs) (bi_later <$> Qs_mut) sch ∗-∗
+  bi_schema_interp lvl (bi_later <$> Ps) (bi_later <$> Ps_mut) sch.
+Proof.
+  iIntros "#HPQ1 #HPQ2".
+  iInduction sch as [] "IH"; rewrite ?bi_schema_interp_unfold; try auto; rewrite //=.
+  - iSplit; iIntros "H"; iSplit;
+    try iApply "IH"; try iApply "IH1"; try iDestruct "H" as "($&_)"; try iDestruct "H" as "(_&$)".
+  - iSplit; iIntros "HQ"; iDestruct "HQ" as "[HQ|HQ]";
+      try (iLeft; by iApply "IH");
+      try (iRight; by iApply "IH1").
+  - iSplit; simpl; iIntros "H"; iIntros (a); iApply "IH"; eauto.
+  - iSplit; simpl; iDestruct 1 as (a) "H"; iExists a; by iApply "IH"; eauto.
+  - iSplit; simpl; iDestruct 1 as "(H1&H2)"; iSplitL "H1"; try (by iApply "IH"); try (by iApply "IH1").
+  - iSplit; simpl; iIntros "Hw H1"; iApply "IH1"; iApply "Hw"; iApply "IH"; auto.
+  - iSplit; simpl; iIntros "#H !>"; iApply "IH"; eauto.
+  - iSplit; simpl; iIntros "H !>"; iApply "IH"; eauto.
+  - iSplit; simpl; iIntros ">H"; iApply "IH"; eauto.
+  - iSpecialize ("HPQ1" $! n). iSplit; rewrite ?list_lookup_fmap;
+    destruct (Qs !! n) as [|] eqn:Heq1; rewrite Heq1 => //=;
+    destruct (Ps !! n) as [|] eqn:Heq2; rewrite Heq2 => //=;
+    iIntros; rewrite option_equivI; auto; iNext.
+    * by iRewrite -"HPQ1".
+    * by iRewrite "HPQ1".
+  - iSpecialize ("HPQ2" $! n). iSplit; rewrite ?list_lookup_fmap;
+    destruct (Qs_mut !! n) as [|] eqn:Heq1; rewrite Heq1 => //=;
+    destruct (Ps_mut !! n) as [|] eqn:Heq2; rewrite Heq2 => //=;
+    iIntros; rewrite option_equivI; auto; iNext.
+    * by iRewrite -"HPQ2".
+    * by iRewrite "HPQ2".
+Qed.
+
+Lemma ownI_open {n} lvl i sch (Ps: vec _ n) :
+  wsat (S lvl) ∗ ownI lvl i sch Ps ∗ ownE {[i]} ⊢
+  wsat (S lvl) ∗ (∃ m (Ps_mut: vec _ m),
+                        bi_schema_interp lvl (bi_later <$> (vec_to_list Ps))
+                                             (bi_later <$> (vec_to_list Ps_mut)) sch ∗
+                        ownI_mut lvl i (1/2)%Qp Ps_mut) ∗ ownD {[i]}.
+Proof.
+  rewrite /ownI wsat_unfold.
+  iIntros "((Hw&$) & Hi & HiE)". iDestruct "Hw" as (I) "[Hw HI]".
+  iDestruct "Hw" as (γs1) "(#Hidx1&Hw)".
+  iDestruct "Hi" as (γs2) "(#Hidx2&Hi)".
+  iDestruct (fmlist_idx_agree_1 with "Hidx1 Hidx2") as %->.
+  iDestruct (invariant_lookup_weak I _ i sch Ps with "[$]") as (Qs Qs_mut HIlookup Hlen) "#HPQ".
+  iDestruct (big_sepM_delete _ _ i with "HI") as "[[[HQ [HQ_mut $]]|HiE'] HI]"; eauto.
+  - iSplitR "HQ HQ_mut"; last first. iExists (length Qs_mut), (list_to_vec Qs_mut). iFrame.
+    { rewrite //=. rewrite vec_to_list_to_vec. iApply (bi_schema_interp_ctx_later with "[HPQ] [] [$]").
+      - iIntros (i0). iNext => //=. by iRewrite -("HPQ" $! i0).
+      - iIntros (i0). iNext => //=.
+    }
+    iExists I. iSplitL "Hw".
+    { by eauto with iFrame. }
+    iApply (big_sepM_delete _ _ i); eauto.
     iFrame "HI"; eauto.
   - iDestruct (ownE_singleton_twice with "[$HiE $HiE']") as %[].
 Qed.
-Lemma ownI_close i P : wsat ∗ ownI i P ∗ ▷ P ∗ ownD {[i]} ⊢ wsat ∗ ownE {[i]}.
+
+Lemma gmap_validI_singleton `{Countable K} {A: cmraT} {M: ucmraT} (i: K) (a: A) :
+  ✓ {[ i := a ]} ⊣⊢@{uPredI M} ✓ a.
 Proof.
-  rewrite /ownI /wsat -!lock.
-  iIntros "(Hw & Hi & HP & HiD)". iDestruct "Hw" as (I) "[Hw HI]".
-  iDestruct (invariant_lookup with "[$]") as (Q ?) "#HPQ".
-  iDestruct (big_sepM_delete _ _ i with "HI") as "[[[HQ ?]|$] HI]"; eauto.
-  - iDestruct (ownD_singleton_twice with "[$]") as %[].
-  - iExists I. iFrame "Hw". iApply (big_sepM_delete _ _ i); eauto.
-    iFrame "HI". iLeft. iFrame "HiD". by iNext; iRewrite "HPQ".
+  rewrite gmap_validI. iSplit.
+  - iIntros "H". iSpecialize ("H" $! i). rewrite lookup_singleton uPred.option_validI //=.
+  - iIntros "Ha". iIntros (j). destruct (decide (i = j)).
+    * subst. rewrite lookup_singleton uPred.option_validI //=.
+    * rewrite lookup_singleton_ne //=.
 Qed.
 
-Lemma ownI_alloc φ P :
-  (∀ E : gset positive, ∃ i, i ∉ E ∧ φ i) →
-  wsat ∗ ▷ P ==∗ ∃ i, ⌜φ i⌝ ∗ wsat ∗ ownI i P.
+Lemma ownI_close {n m} lvl i sch (Ps : vec _ n) (Ps_mut: vec _ m) :
+  wsat (S lvl) ∗
+  ownI lvl i sch Ps ∗
+  ownI_mut lvl i (1/2)%Qp Ps_mut ∗
+  bi_schema_interp lvl (bi_later <$> (vec_to_list Ps)) (bi_later <$> (vec_to_list Ps_mut)) sch ∗
+  ownD {[i]} ⊢
+  wsat (S lvl) ∗ ownE {[i]}.
 Proof.
-  iIntros (Hfresh) "[Hw HP]". rewrite /wsat -!lock.
+  rewrite /ownI wsat_unfold.
+  iIntros "((Hw&$) & Hi & Hi_mut & HP & HiD)". iDestruct "Hw" as (I) "[Hw HI]".
+  iDestruct "Hw" as (γs1) "(#Hidx1&Hw)".
+  iDestruct "Hi" as (γs2) "(#Hidx2&Hi)".
+  iEval (rewrite /ownI_mut) in "Hi_mut".
+  iDestruct "Hi_mut" as (? γs2_mut) "(#Hidx3&Hi_mut)".
+  iDestruct (fmlist_idx_agree_1 with "Hidx1 Hidx2") as %->.
+  iDestruct (fmlist_idx_agree_1 with "Hidx3 Hidx2") as %->.
+  iDestruct (invariant_lookup_strong with "[$Hw Hi Hi_mut]")
+    as (Qs Qs_mut HIlookup Hlen Hlen_mut) "(#HPQ&#HPQ_mut)".
+  { iCombine "Hi Hi_mut" as "Hcombine".
+    iDestruct (own_valid with "Hcombine") as "#Hval".
+    rewrite auth_validI /= gmap_validI_singleton uPred.prod_validI /=.
+    rewrite agree_validI. iDestruct "Hval" as "(Hval_agree&_)".
+    iRewrite -"Hval_agree" in "Hcombine".
+    rewrite agree_idemp left_id. eauto.
+  }
+  iDestruct (big_sepM_delete _ _ i with "HI") as "[[[HQ [HQmut ?]]|$] HI]"; eauto.
+  - iDestruct (ownD_singleton_twice with "[$]") as %[].
+  - iExists I. iSplitL "Hw".
+    { by eauto with iFrame. }
+    iApply (big_sepM_delete _ _ i); eauto.
+    iFrame "HI". iLeft. iFrame "HiD". iClear "Hi".
+    iSplitL "HP".
+    { by iApply (bi_schema_interp_ctx_later with "HPQ HPQ_mut"). }
+    iApply (ownI_mut_later _ _ _ Ps_mut (list_to_vec Qs_mut)).
+    { rewrite -(vec_to_list_length Ps_mut). auto. }
+    { iIntros (j). rewrite vec_to_list_to_vec. iNext. by iRewrite ("HPQ_mut" $! j). }
+    iExists _, _. iFrame "Hidx2"; eauto.
+Qed.
+
+Lemma ownI_mut_update {m m'} γ (i: positive) I x
+      (Qs_mut: vec (iProp Σ) m) (Qs_mut': vec (iProp Σ) m') :
+  own γ (● (inv_cmra_fmap <$> I : gmap _ _)) -∗
+  own γ (◯ {[i := (x, inv_mut_unfold 1%Qp Qs_mut)]}) ==∗
+  ∃ PsI schI QsI (Hlook: I !! i = Some ((PsI, schI), QsI)),
+  own γ (● (inv_cmra_fmap <$> (<[i := ((PsI, schI), vec_to_list Qs_mut')]> I) : gmap _ _)) ∗
+  own γ (◯ {[i := (x, inv_mut_unfold 1%Qp Qs_mut')]}).
+Proof.
+  iIntros "Hauth Hfrag".
+  iDestruct (own_valid_2 with "Hauth Hfrag")
+      as "#Hval".
+  (* This is more complicated than something like gen_heap_update, because we cannot eliminate
+     the validity to a pure fact. *)
+  destruct (I !! i) as [((QsI&schI)&Qs_mutI)|] eqn:Hlookup; last first.
+  {
+    rewrite auth_both_validI.
+    iDestruct "Hval" as "(_&Hval&_)".
+    iDestruct "Hval" as (I') "Heq".
+    rewrite gmap_equivI. iSpecialize ("Heq" $! i). rewrite lookup_fmap Hlookup //=.
+    rewrite lookup_op lookup_singleton option_equivI.
+    case (I' !! i) => //=.
+  }
+  iExists QsI, schI, Qs_mutI.
+  iMod (own_update_2 with "Hauth Hfrag") as "[$ $]"; last done.
+  { eapply auth_update. rewrite fmap_insert. eapply singleton_local_update.
+    { rewrite lookup_fmap Hlookup //=. }
+    apply prod_local_update.
+    { rewrite //=. }
+    { rewrite /= /inv_mut_unfold //=. rewrite ?vec_to_list_to_vec.
+      apply option_local_update.
+      apply exclusive_local_update => //=.
+    }
+  }
+Qed.
+
+Lemma ownI_full_split_frac γ x i q {n} (Ps_mut: vec _ n):
+  own γ (◯ {[i := (x, inv_mut_unfold q Ps_mut)]}) -∗
+  own γ (◯ {[i := (x, inv_mut_unfold (q/2) Ps_mut)]}) ∗
+  own γ (◯ {[i := (x, inv_mut_unfold (q/2) Ps_mut)]}).
+Proof.
+  rewrite -own_op. iIntros "H". iApply (own_proper with "H").
+  apply auth_frag_proper => //=.
+  intros j. rewrite lookup_op. destruct (decide (i = j)); last first.
+  { rewrite ?lookup_singleton_ne //=. }
+  subst. rewrite ?lookup_singleton /=.
+  rewrite -Some_op -pair_op agree_idemp /inv_mut_unfold.
+  rewrite -Some_op -pair_op agree_idemp.
+  repeat f_equiv. by rewrite frac_op' Qp_div_2.
+Qed.
+
+Lemma ownI_full_split_comp γ x y i:
+  own γ (◯ {[i := (x, y)]}) -∗
+  own γ (◯ {[i := (x, ε)]}) ∗
+  own γ (◯ {[i := (x, y)]}).
+Proof.
+  rewrite -own_op. iIntros "H". iApply (own_proper with "H").
+  apply auth_frag_proper => //=.
+  intros j. rewrite lookup_op. destruct (decide (i = j)); last first.
+  { rewrite ?lookup_singleton_ne //=. }
+  subst. rewrite ?lookup_singleton /=.
+  rewrite -Some_op -pair_op agree_idemp /inv_mut_unfold left_id //=.
+Qed.
+
+Lemma ownI_mut_agree {n m} lvl i q1 q2 (Qs_mut1: vec _ n) (Qs_mut2: vec _ m):
+  ownI_mut lvl i q1 Qs_mut1 -∗
+  ownI_mut lvl i q2 Qs_mut2 -∗
+  ⌜ n = m ⌝ ∗ (∀ j, ▷ (vec_to_list Qs_mut1 !! j ≡  vec_to_list Qs_mut2 !! j)).
+Proof.
+  rewrite /ownI_mut.
+  iDestruct 1 as (l1 γs1) "(#Hidx1&Hown1)".
+  iDestruct 1 as (l2 γs2) "(#Hidx2&Hown2)".
+  iDestruct (fmlist_idx_agree_1 with "Hidx1 Hidx2") as %->.
+  iCombine "Hown1 Hown2" as "Hown".
+  iDestruct (own_valid with "Hown") as "Hval".
+  rewrite auth_validI /= gmap_validI.
+  iSpecialize ("Hval" $! i).
+  rewrite lookup_singleton /= uPred.option_validI /= uPred.prod_validI /=.
+  iDestruct "Hval" as "(_&Hval)".
+  rewrite uPred.option_validI /= uPred.prod_validI /=.
+  iDestruct "Hval" as "(_&Hagree)".
+  rewrite agree_validI agree_equivI.
+  (* XXX: this pattern is repeated a few times in other proofs. prove a lemma *)
+  iDestruct (list_equivI_length with "Hagree") as %Hlen.
+  iSplitL "".
+  { iPureIntro. rewrite ?fmap_length ?vec_to_list_length //= in Hlen. }
+  rewrite ?list_equivI_1. iIntros (j). iSpecialize ("Hagree" $! j).
+  rewrite ?list_lookup_fmap ?vec_to_list_to_vec.
+  rewrite option_equivI.
+  destruct (vec_to_list Qs_mut1 !! j) as [Q0|] eqn:HeqQ;
+  destruct (vec_to_list Qs_mut2 !! j) as [P0|] eqn:HeqP;
+  rewrite ?HeqQ ?HeqP //=.
+  rewrite //= ?later_equivI iProp_unfold_equivI //=. iNext. by iRewrite "Hagree".
+Qed.
+
+Lemma ownI_mut_combine {n m} lvl i q1 q2 (Qs_mut1: vec _ n) (Qs_mut2: vec _ m):
+  ownI_mut lvl i q1 Qs_mut1 -∗
+  ownI_mut lvl i q2 Qs_mut2 -∗
+  ownI_mut lvl i (q1 + q2)%Qp Qs_mut1.
+Proof.
+  rewrite /ownI_mut.
+  iDestruct 1 as (l1 γs1) "(#Hidx1&Hown1)".
+  iDestruct 1 as (l2 γs2) "(#Hidx2&Hown2)".
+  iDestruct (fmlist_idx_agree_1 with "Hidx1 Hidx2") as %->.
+  iExists l1, _.  iFrame "Hidx1".
+  iCombine "Hown1 Hown2" as "Hown".
+  iDestruct (own_valid with "Hown") as "#Hval".
+  rewrite auth_validI /= gmap_validI.
+  iSpecialize ("Hval" $! i).
+  rewrite lookup_singleton /= uPred.option_validI /= uPred.prod_validI /=.
+  iDestruct "Hval" as "(Hval1&Hval2)".
+  rewrite agree_op_invI. iRewrite -"Hval1" in "Hown".
+  rewrite agree_idemp.
+  rewrite /= uPred.option_validI /= uPred.prod_validI /=.
+  iDestruct "Hval2" as "(Hval2a&Hval2b)".
+  rewrite agree_op_invI. iRewrite -"Hval2b" in "Hown".
+  rewrite agree_idemp.
+  eauto.
+Qed.
+
+Lemma ownI_close_modify {n m m'} lvl i sch (Ps : vec _ n) (Ps_mut: vec _ m) (Qs_mut: vec _ m') :
+  wsat (S lvl) ∗
+  ownI lvl i sch Ps ∗
+  ownI_mut lvl i 1%Qp Qs_mut ∗
+  bi_schema_interp lvl (bi_later <$> (vec_to_list Ps)) (bi_later <$> (vec_to_list Ps_mut)) sch ∗
+  ownD {[i]} ⊢
+  |==> wsat (S lvl) ∗ ownE {[i]} ∗ ownI_mut lvl i (1/2)%Qp Ps_mut.
+Proof.
+  rewrite /ownI wsat_unfold.
+  iIntros "((Hw&$) & Hi & Hi_mut & HP & HiD)". iDestruct "Hw" as (I) "[Hw HI]".
+  iDestruct "Hw" as (γs1) "(#Hidx1&Hw)".
+  iDestruct "Hi" as (γs2) "(#Hidx2&Hi)".
+  iEval (rewrite /ownI_mut) in "Hi_mut".
+  iDestruct "Hi_mut" as (? γs2_mut) "(#Hidx3&Hi_mut)".
+  iDestruct (fmlist_idx_agree_1 with "Hidx1 Hidx2") as %->.
+  iDestruct (fmlist_idx_agree_1 with "Hidx3 Hidx2") as %->.
+  iDestruct (invariant_lookup_strong with "[$Hw Hi Hi_mut]")
+    as (Qs' Qs_mut' HIlookup Hlen Hlen_mut) "(#HPQ&#HPQ_mut)".
+  { iCombine "Hi Hi_mut" as "Hcombine".
+    iDestruct (own_valid with "Hcombine") as "#Hval".
+    rewrite auth_validI /= gmap_validI_singleton uPred.prod_validI /=.
+    rewrite agree_validI. iDestruct "Hval" as "(Hval_agree&_)".
+    iRewrite -"Hval_agree" in "Hcombine".
+    rewrite agree_idemp left_id. eauto.
+  }
+  iDestruct (big_sepM_insert_acc _ _ i with "HI") as "[[[HQ [HQmut ?]]|$] HI]"; eauto.
+  { iDestruct (ownD_singleton_twice with "[$]") as %[]. }
+  iMod (ownI_mut_update _ _ _ _ _ Ps_mut with "[$] [$]") as (Ps' sch' ? HIlookup') "(Hw&Hi_mut)".
+  iModIntro. iDestruct (ownI_full_split_frac with "Hi_mut") as "(Hi_mut1&Hi_mut2)".
+  iSplitR "Hi_mut2"; last first.
+  { iExists _, _. by iFrame. }
+  iExists _.
+  iSplitL "Hw".
+  { by eauto with iFrame. }
+  iApply "HI". iLeft.
+  iFrame "HiD". iClear "Hi".
+  iSplitL "HP".
+  { simpl. rewrite HIlookup in HIlookup'. inversion HIlookup'; subst.
+    iApply (bi_schema_interp_ctx_later with "HPQ []"); last eauto.
+    { iIntros; iNext. trivial. }
+  }
+  iExists _, _. iFrame "Hidx2" => /=. rewrite /inv_mut_unfold vec_to_list_to_vec //=.
+Qed.
+
+Lemma ownI_alloc {n m} φ sch lvl (Ps: vec _ n) (Ps_mut: vec _ m):
+  (∀ E : gset positive, ∃ i, i ∉ E ∧ φ i) →
+  wsat (S lvl) ∗
+  bi_schema_interp lvl (bi_later <$> (vec_to_list Ps)) (bi_later <$> (vec_to_list Ps_mut)) sch ==∗
+  ∃ i, ⌜φ i⌝ ∗ wsat (S lvl) ∗ ownI lvl i sch Ps ∗ ownI_mut lvl i (1/2)%Qp Ps_mut.
+Proof.
+  rewrite wsat_unfold.
+  iIntros (Hfresh) "[(Hw&$) HP]".
   iDestruct "Hw" as (I) "[Hw HI]".
+  iDestruct "Hw" as (γs) "(#Hidx1&Hw)".
   iMod (own_unit (gset_disjUR positive) disabled_name) as "HE".
   iMod (own_updateP with "[$]") as "HE".
   { apply (gset_disj_alloc_empty_updateP_strong' (λ i, I !! i = None ∧ φ i)).
@@ -160,20 +772,46 @@ Proof.
   iDestruct "HE" as (X) "[Hi HE]"; iDestruct "Hi" as %(i & -> & HIi & ?).
   iMod (own_update with "Hw") as "[Hw HiP]".
   { eapply auth_update_alloc,
-     (alloc_singleton_local_update _ i (invariant_unfold P)); last done.
+     (alloc_singleton_local_update _ i (invariant_unfold sch Ps, inv_mut_unfold 1%Qp Ps_mut)); last done.
     by rewrite /= lookup_fmap HIi. }
-  iModIntro; iExists i;  iSplit; [done|]. rewrite /ownI; iFrame "HiP".
-  iExists (<[i:=P]>I); iSplitL "Hw".
-  { by rewrite fmap_insert insert_singleton_op ?lookup_fmap ?HIi. }
+  iDestruct (ownI_full_split_comp with "HiP") as "(Hi_pers&Hi_mut)".
+  iDestruct (ownI_full_split_frac with "Hi_mut") as "(Hi_mut1&Hi_mut2)".
+  iModIntro; iExists i;  iSplit; [done|]. iSplitR "Hi_pers Hi_mut1"; last first.
+  { rewrite /ownI/ownI_mut. iSplitL "Hi_pers".
+    { iExists _; iFrame "Hidx1"; eauto. }
+    { iExists _, _; iFrame "Hidx1"; eauto. }
+  }
+  iExists (<[i:=((vec_to_list Ps, sch), vec_to_list Ps_mut)]>I); iSplitL "Hw".
+  { iExists γs. iFrame "Hidx1".
+    rewrite ?fmap_insert ?insert_singleton_op ?lookup_fmap ?HIi //=
+            /invariant_unfold/inv_mut_unfold ?vec_to_list_to_vec //=. }
   iApply (big_sepM_insert _ I); first done.
-  iFrame "HI". iLeft. by rewrite /ownD; iFrame.
+  iFrame "HI". iLeft. rewrite /ownD. iFrame.
+  iExists _, _. iFrame "Hidx1". rewrite /inv_mut_unfold ?vec_to_list_to_vec //=.
 Qed.
 
-Lemma ownI_alloc_open φ P :
+Lemma ownI_alloc_nomut {n} φ sch lvl (Ps: vec _ n):
   (∀ E : gset positive, ∃ i, i ∉ E ∧ φ i) →
-  wsat ==∗ ∃ i, ⌜φ i⌝ ∗ (ownE {[i]} -∗ wsat) ∗ ownI i P ∗ ownD {[i]}.
+  wsat (S lvl) ∗
+  bi_schema_interp lvl (bi_later <$> (vec_to_list Ps)) [] sch ==∗
+  ∃ i, ⌜φ i⌝ ∗ wsat (S lvl) ∗ ownI lvl i sch Ps.
 Proof.
-  iIntros (Hfresh) "Hw". rewrite /wsat -!lock. iDestruct "Hw" as (I) "[Hw HI]".
+  iIntros. iMod (ownI_alloc _ _ _ _ (list_to_vec []) with "[$]") as (?) "(?&?&?&?)"; auto.
+Qed.
+
+Lemma ownI_alloc_open {n m} lvl φ sch (Ps: vec _ n) (Ps_mut : vec _ m) :
+  (∀ E : gset positive, ∃ i, i ∉ E ∧ φ i) →
+  wsat (S lvl) ==∗
+  ∃ i, ⌜φ i⌝ ∗
+       (ownE {[i]} -∗ wsat (S lvl)) ∗
+       ownI lvl i sch Ps ∗
+       ownI_mut lvl i (1/2)%Qp Ps_mut ∗
+       ownD {[i]}.
+Proof.
+  iIntros (Hfresh) "Hw". rewrite wsat_unfold.
+  iDestruct "Hw" as "(Hw&$)".
+  iDestruct "Hw" as (I) "[Hw HI]".
+  iDestruct "Hw" as (γs) "(#Hidx1&Hw)".
   iMod (own_unit (gset_disjUR positive) disabled_name) as "HD".
   iMod (own_updateP with "[$]") as "HD".
   { apply (gset_disj_alloc_empty_updateP_strong' (λ i, I !! i = None ∧ φ i)).
@@ -182,26 +820,280 @@ Proof.
   iDestruct "HD" as (X) "[Hi HD]"; iDestruct "Hi" as %(i & -> & HIi & ?).
   iMod (own_update with "Hw") as "[Hw HiP]".
   { eapply auth_update_alloc,
-     (alloc_singleton_local_update _ i (invariant_unfold P)); last done.
+     (alloc_singleton_local_update _ i (invariant_unfold sch Ps, inv_mut_unfold 1%Qp Ps_mut)); last done.
     by rewrite /= lookup_fmap HIi. }
-  iModIntro; iExists i;  iSplit; [done|]. rewrite /ownI; iFrame "HiP".
-  rewrite -/(ownD _). iFrame "HD".
-  iIntros "HE". iExists (<[i:=P]>I); iSplitL "Hw".
-  { by rewrite fmap_insert insert_singleton_op ?lookup_fmap ?HIi. }
+  iDestruct (ownI_full_split_comp with "HiP") as "(Hi_pers&Hi_mut)".
+  iDestruct (ownI_full_split_frac with "Hi_mut") as "(Hi_mut1&Hi_mut2)".
+  iModIntro; iExists i;  iSplit; [done|]. iSplitR "Hi_pers Hi_mut1 HD"; last first.
+  { rewrite /ownI/ownI_mut. iSplitL "Hi_pers".
+    { iExists _; iFrame "Hidx1"; eauto. }
+    iSplitL "Hi_mut1".
+    { iExists _, _; iFrame "Hidx1"; eauto. }
+    rewrite /ownD; eauto.
+  }
+  iIntros "HE".
+  iExists (<[i:=((vec_to_list Ps, sch), vec_to_list Ps_mut)]>I); iSplitL "Hw".
+  { iExists γs. iFrame "Hidx1".
+    rewrite ?fmap_insert ?insert_singleton_op ?lookup_fmap ?HIi //=
+            /invariant_unfold/inv_mut_unfold ?vec_to_list_to_vec //=. }
   iApply (big_sepM_insert _ I); first done.
   iFrame "HI". by iRight.
 Qed.
+
+Lemma wsat_alloc_new_level l:
+  wsat (length l) -∗ fmlist (inv_list_name) 1 l ==∗
+  ∃ (γ: invariant_level_names), fmlist inv_list_name 1 (l ++ [γ]) ∗ wsat (S (length l)).
+Proof.
+  iIntros "Hw Hlist".
+  rewrite ?wsat_unfold. iFrame.
+  iMod (own_alloc (● (∅ : gmap positive _))) as (γ) "HI";
+    first by rewrite auth_auth_valid.
+  iExists {| invariant_name := γ |}.
+  iMod (fmlist_update (l ++ [{| invariant_name := γ|}]) with "[$]") as "($&Hidx)".
+  { eexists; eauto. }
+  iModIntro.
+  iExists ∅. rewrite fmap_empty big_sepM_empty right_id.
+  iExists {| invariant_name := γ |}; iFrame.
+  iApply fmlist_lb_to_idx; auto.
+  rewrite lookup_app_r //=. replace (length l - length l) with O by lia; auto.
+Qed.
+
+Lemma wsat_alloc_new_levels l n:
+  wsat (length l) -∗ fmlist (inv_list_name) 1 l ==∗
+  ∃ l', ⌜ length l' = n ⌝ ∗ fmlist inv_list_name 1 (l ++ l') ∗ wsat (length (l ++ l')).
+Proof.
+  iIntros "Hw Hlist".
+  iInduction n as [| n] "IH".
+  - iModIntro; iExists []. rewrite ?right_id. by iFrame.
+  - iMod ("IH" with "[$] [$]") as (l' Hlen) "(Hw&Hlist)".
+    iMod (wsat_alloc_new_level with "[$] [$]") as (γ) "(Hlist&Hw)".
+    iExists (l' ++ [γ]). rewrite ?app_length //=.
+    rewrite app_assoc. iFrame.
+    replace (length l + (length l' + 1)) with (S (length l + length l')) by lia; iFrame.
+    iPureIntro. lia.
+Qed.
+
+Definition wsat_all := (∃ l, wsat (length l) ∗ fmlist (inv_list_name) 1 l)%I.
+
+Lemma wsat_all_acc n:
+  wsat_all ==∗ wsat n ∗ (wsat n -∗ wsat_all).
+Proof.
+  iDestruct 1 as (l) "(Hw&Hlist)".
+  iMod (wsat_alloc_new_levels l (n - length l) with "[$] [$]") as (l' Hlen) "(Hlist&Hw)".
+  iDestruct (wsat_le_acc n with "[$]") as "($&Hclo)"; first auto.
+  { rewrite app_length. lia. }
+  iIntros "!> Hw". iExists _. iFrame. by iApply "Hclo".
+Qed.
+
 End wsat.
 
 (* Allocation of an initial world *)
-Lemma wsat_alloc `{!invPreG Σ} : ⊢ |==> ∃ _ : invG Σ, wsat ∗ ownE ⊤.
+Lemma wsat_alloc' `{!invPreG Σ} :
+  ⊢ |==> ∃ (_ : invG Σ), wsat_all ∗ ownE ⊤.
 Proof.
   iIntros.
-  iMod (own_alloc (● (∅ : gmap positive _))) as (γI) "HI";
-    first by rewrite auth_auth_valid.
+  iMod (fmlist_alloc []) as (γI) "HI".
   iMod (own_alloc (CoPset ⊤)) as (γE) "HE"; first done.
   iMod (own_alloc (GSet ∅)) as (γD) "HD"; first done.
-  iModIntro; iExists (WsatG _ _ _ _ γI γE γD).
-  rewrite /wsat /ownE -lock; iFrame.
-  iExists ∅. rewrite fmap_empty big_opM_empty. by iFrame.
+  set (iG := (WsatG _ _ _ _ _ γI γE γD)).
+  iExists iG.
+  rewrite /ownE. iFrame. iClear "HD".
+  replace γI with (inv_list_name) by eauto.
+  iExists [] => //=. iFrame. rewrite wsat_unfold //.
 Qed.
+
+Lemma wsat_alloc `{!invPreG Σ} n : ⊢ |==> ∃ _ : invG Σ, wsat n ∗ ownE ⊤.
+Proof.
+  iIntros.
+  iMod (wsat_alloc') as (?) "(Hall&Hown)".
+  iExists _. iMod (wsat_all_acc n with "[$]") as "(?&?)".
+  by iFrame.
+Qed.
+
+Section schema_test_bupd.
+Context `{!invG Σ}.
+Implicit Types P : iProp Σ.
+
+Definition ownI_bupd lvl i P := ownI lvl i (bi_sch_bupd (bi_sch_var_fixed O)) (list_to_vec [P]).
+
+Lemma ownI_bupd_alloc lvl φ P :
+  (∀ E : gset positive, ∃ i, i ∉ E ∧ φ i) →
+  wsat (S lvl) ∗ (|==> ▷ P) ==∗ ∃ i, ⌜φ i⌝ ∗ wsat (S lvl) ∗ ownI_bupd lvl i P.
+Proof.
+  iIntros (?) "HwP".
+  iApply (ownI_alloc_nomut); auto.
+  rewrite ?bi_schema_interp_unfold //=.
+Qed.
+
+Lemma ownI_bupd_open lvl i P :
+  wsat (S lvl) ∗ ownI_bupd lvl i P ∗ ownE {[i]} ⊢ wsat (S lvl) ∗ |==> ▷ P ∗ ownD {[i]}.
+Proof.
+ iIntros "Hw".
+ iDestruct (ownI_open with "Hw") as "($&HP&$)".
+ iDestruct "HP" as (??) "(HP&_)".
+ rewrite ?bi_schema_interp_unfold //=.
+Qed.
+
+End schema_test_bupd.
+
+Section schema_test_fupd.
+Context `{!invG Σ}.
+Implicit Types P : iProp Σ.
+
+Definition bi_sch_False : bi_schema := bi_sch_pure False.
+
+Definition bi_sch_except_0 (P: bi_schema) : bi_schema :=
+  bi_sch_or (bi_sch_later (bi_sch_False)) P.
+
+Definition bi_sch_bupd_wand (P1 P2: bi_schema) :=
+  bi_sch_wand P1 (bi_sch_bupd P2).
+
+Definition bi_sch_fupd E1 E2 (P: bi_schema) : bi_schema :=
+  bi_sch_bupd_wand
+    (bi_sch_sep (bi_sch_wsat) (bi_sch_ownE E1))
+    (bi_sch_except_0 (bi_sch_sep (bi_sch_wsat)
+                                (bi_sch_sep (bi_sch_ownE E2) P))).
+
+Lemma bi_sch_fupd_interp E1 E2 lvl Qs Qs_mut Psch P:
+  bi_schema_interp lvl Qs Qs_mut Psch = P →
+  bi_schema_interp lvl Qs Qs_mut (bi_sch_fupd E1 E2 Psch) =
+    (wsat lvl ∗ ownE E1 ==∗ ◇ (wsat lvl ∗ ownE E2 ∗ P))%I.
+Proof.
+  intros Heq.
+  rewrite ?bi_schema_interp_unfold //=.
+  do 11 (rewrite {1}bi_schema_interp_unfold //=).
+  rewrite Heq. rewrite ?bi_schema_interp_unfold //=.
+Qed.
+
+Definition ownI_fupd lvl i E1 E2 P :=
+  ownI lvl i (bi_sch_fupd E1 E2 (bi_sch_var_fixed O)) (list_to_vec [P]).
+
+Lemma ownI_fupd_alloc lvl E1 E2 φ P :
+  (∀ E : gset positive, ∃ i, i ∉ E ∧ φ i) →
+  wsat (S lvl) ∗ (wsat lvl ∗ ownE E1 ==∗ ◇ (wsat lvl ∗ ownE E2 ∗ ▷ P))
+       ==∗ ∃ i, ⌜φ i⌝ ∗ wsat (S lvl) ∗ ownI_fupd lvl i E1 E2 P.
+Proof.
+  iIntros (?) "HwP". iApply ownI_alloc_nomut; eauto.
+  erewrite bi_sch_fupd_interp; eauto.
+  rewrite ?bi_schema_interp_unfold //=.
+Qed.
+
+Lemma ownI_fupd_open lvl E1 E2 i P :
+  wsat (S lvl) ∗ ownI_fupd lvl i E1 E2 P ∗ ownE {[i]} ⊢
+  wsat (S lvl) ∗ (wsat lvl ∗ ownE E1 ==∗ ◇ (wsat lvl ∗ ownE E2 ∗ ▷ P)) ∗ ownD {[i]}.
+Proof.
+  iIntros "Hw". iDestruct (ownI_open with "Hw") as "($&HP&$)".
+  iDestruct "HP" as (??) "(HP&_)".
+  erewrite bi_sch_fupd_interp; eauto.
+  rewrite ?bi_schema_interp_unfold //=.
+Qed.
+
+End schema_test_fupd.
+
+Section schema_test_mut.
+Context `{!invG Σ}.
+Implicit Types P Q : iProp Σ.
+
+Definition bi_sch_bupd_factory (Q P: bi_schema) : bi_schema :=
+  bi_sch_sep Q (bi_sch_persistently (bi_sch_wand Q (bi_sch_bupd (bi_sch_sep Q P)))).
+
+Definition ownI_bupd_factory lvl i P :=
+  ownI lvl i (bi_sch_bupd_factory (bi_sch_var_mut O) (bi_sch_var_fixed O)) (list_to_vec [P]).
+
+Definition ownI_full_bupd_factory lvl i q Q P :=
+  (∃ n (Qs: vec _ n), ownI lvl i (bi_sch_bupd_factory (bi_sch_var_mut O) (bi_sch_var_fixed O)) (list_to_vec [P]) ∗
+   ownI_mut lvl i q Qs ∗ ⌜ default True%I (vec_to_list Qs !! 0) = Q ⌝)%I.
+
+Lemma ownI_bupd_factory_alloc lvl φ Q P :
+  (∀ E : gset positive, ∃ i, i ∉ E ∧ φ i) →
+  wsat (S lvl) ∗ (▷ Q ∗ □ (▷ Q ==∗ ▷ Q ∗ ▷ P))
+       ==∗ ∃ i, ⌜φ i⌝ ∗ wsat (S lvl) ∗ ownI_full_bupd_factory lvl i (1/2)%Qp Q P.
+Proof.
+  iIntros (?) "(Hw&(HQ&#Hfactory))". iMod (ownI_alloc with "[$Hw HQ]") as (i) "(?&?&?&?)"; eauto; last first.
+  { iModIntro. iExists i. iFrame. iExists 1, (list_to_vec [Q]). iFrame. rewrite //=. }
+  repeat (rewrite ?bi_schema_interp_unfold //=).
+  iFrame. eauto.
+Qed.
+
+Lemma ownI_full_bupd_factory_open lvl i Q P:
+  wsat (S lvl) ∗ ownI_full_bupd_factory lvl i (1/2)%Qp Q P ∗ ownE {[i]} ⊢
+  wsat (S lvl) ∗ (▷ Q ∗ □ (▷ Q ==∗ ▷ Q ∗ ▷ P)) ∗ ownI_full_bupd_factory lvl i 1%Qp Q P ∗ ownD {[i]}.
+Proof.
+  iIntros "(Hw&Hfull&HE)".
+  iDestruct "Hfull" as (? Qs) "(#HI&HI_mut&Hp)".
+  iDestruct "Hp" as %Hp.
+  iPoseProof (ownI_open with "[$Hw $HI $HE]") as "($&H&$)".
+  iDestruct "H" as (??) "(Hinterp&HI_mut2)".
+  iDestruct (ownI_mut_agree with "HI_mut HI_mut2") as (Hlen) "#Hequiv".
+  iDestruct (bi_schema_interp_ctx_later with "[] Hequiv Hinterp") as "Hinterp".
+  { iIntros. iNext. eauto. }
+  repeat (rewrite ?bi_schema_interp_unfold //=).
+  iSplitL "Hinterp".
+  rewrite ?list_lookup_fmap.
+  { destruct (vec_to_list Qs !! 0) as [?|] eqn:Heq. rewrite ?Heq => //=.
+    * move: Hp => //= ->.
+      { iDestruct "Hinterp" as "($&#$)". }
+    * move: Hp. rewrite Heq => //= <-.
+      { iDestruct "Hinterp" as "(?&#Hwand)". iSplitL ""; first eauto.
+        iModIntro. iIntros. iMod ("Hwand" with "[//]") as "(?&$)"; eauto. }
+   }
+  iExists _, _. iFrame "#".
+  iDestruct (ownI_mut_combine with "HI_mut [$]") as "H". rewrite Qp_div_2 //=. iFrame. eauto.
+Qed.
+
+Lemma ownI_bupd_factory_open lvl i P:
+  wsat (S lvl) ∗ ownI_bupd_factory lvl i P ∗ ownE {[i]} ⊢
+  wsat (S lvl) ∗ ∃ Q, (▷ Q ∗ □ (▷ Q ==∗ ▷ Q ∗ ▷ P)) ∗ ownI_full_bupd_factory lvl i (1/2)%Qp Q P ∗ ownD {[i]}.
+Proof.
+  iIntros "(Hw&#HI0&HE)".
+  iPoseProof (ownI_open with "[$Hw $HI0 $HE]") as "($&H&$)".
+  iDestruct "H" as (? Qs_mut) "(Hinterp&HI_mut2)".
+  iExists (default True%I (vec_to_list Qs_mut !! 0)).
+  repeat (rewrite ?bi_schema_interp_unfold //=).
+  rewrite ?list_lookup_fmap.
+  destruct (vec_to_list Qs_mut !! 0) as [?|] eqn:Heq; rewrite Heq //=.
+  - iSplitL "Hinterp".
+    { iDestruct "Hinterp" as "($&#$)". }
+    iFrame "#". iExists _, Qs_mut. rewrite Heq //=. by iFrame.
+  - iSplitL "Hinterp".
+    { iDestruct "Hinterp" as "(?&#Hwand)". iSplitL ""; first eauto.
+      iModIntro. iIntros. iMod ("Hwand" with "[//]") as "(?&$)"; eauto. }
+    iFrame "#". iExists _, Qs_mut. rewrite Heq //=. by iFrame.
+Qed.
+
+Lemma ownI_bupd_factory_close lvl i Q P:
+  wsat (S lvl) ∗ (▷ Q ∗ □ (▷ Q ==∗ ▷ Q ∗ ▷ P)) ∗ ownI_full_bupd_factory lvl i (1/2)%Qp Q P ∗ ownD {[i]} ⊢
+  wsat (S lvl) ∗ ownE {[i]}.
+Proof.
+  iIntros "(Hw&Hinterp&HI0&HD)".
+  iDestruct ("HI0") as (? Qs_mut) "(?&?&Hp)".
+  iDestruct "Hp" as %Hp.
+  iApply (ownI_close).
+  iFrame.
+  repeat (rewrite ?bi_schema_interp_unfold //=).
+  rewrite ?list_lookup_fmap.
+  destruct (vec_to_list Qs_mut !! 0) as [?|] eqn:Heq; rewrite Heq //=.
+  - move: Hp => //= ->.
+    { iDestruct "Hinterp" as "($&#$)". }
+  - move: Hp => //= <-.
+    { iDestruct "Hinterp" as "(?&#Hwand)". iSplitL ""; first eauto.
+      iModIntro. iIntros. iMod ("Hwand" with "[//]") as "(?&$)"; eauto. }
+Qed.
+
+Lemma ownI_bupd_factory_close_modify lvl i Q Q0 P:
+  wsat (S lvl) ∗ (▷ Q ∗ □ (▷ Q ==∗ ▷ Q ∗ ▷ P)) ∗ ownI_full_bupd_factory lvl i 1%Qp Q0 P ∗ ownD {[i]} ⊢
+  |==> wsat (S lvl) ∗ ownE {[i]} ∗ ownI_full_bupd_factory lvl i (1/2)%Qp Q P.
+Proof.
+  iIntros "(Hw&Hinterp&HI0&HD)".
+  iDestruct ("HI0") as (? Qs_mut) "(#Hi&?&Hp)".
+  iDestruct "Hp" as %Hp.
+  iMod (ownI_close_modify _ _ _ _ (list_to_vec [Q]) Qs_mut  with "[-]") as "($&$&?)".
+  {
+    iFrame. iFrame "#".
+    repeat (rewrite ?bi_schema_interp_unfold //=).
+    iDestruct "Hinterp" as "($&#$)".
+  }
+  iExists _, _. iFrame "# ∗" => //=.
+Qed.
+
+End schema_test_mut.
