theories/base_logic/lib/fupd_level.v
@@ -1,0 +1,364 @@
+From stdpp Require Export coPset.
+From iris.proofmode Require Import tactics.
+From iris.algebra Require Import gmap auth agree gset coPset.
+From iris.base_logic.lib Require Export own.
+From iris.base_logic.lib Require Import wsat fancy_updates.
+Set Default Proof Using "Type".
+Export invG.
+Import uPred.
+
+(* This is essentially fancy_updates.v from Iris, but replacing the use of except_0 with atleast *)
+
+Definition uPred_fupd_level_def `{!invG Σ} (E1 E2 : coPset) (k : nat) (P : iProp Σ) : iProp Σ :=
+  wsat (S k) ∗ ownE E1 ==∗ ◇ (wsat (S k) ∗ ownE E2 ∗ P).
+Definition uPred_fupd_level_aux `{!invG Σ} : seal uPred_fupd_level_def. Proof. by eexists. Qed.
+Definition uPred_fupd_level `{!invG Σ} := uPred_fupd_level_aux.(unseal).
+Definition uPred_fupd_level_eq `{!invG Σ} : uPred_fupd_level = uPred_fupd_level_def :=
+  uPred_fupd_level_aux.(seal_eq).
+
+Reserved Notation "| k ={ E1 }=> Q"
+  (at level 99, E1, k at level 50, Q at level 200,
+   format "| k ={ E1 }=>  Q").
+Reserved Notation "| k ={ E1 , E2 }=> Q"
+  (at level 99, E1, E2, k at level 50, Q at level 200,
+   format "| k ={ E1 , E2 }=>  Q").
+Reserved Notation "P = k ={ E1 , E2 }=∗ Q"
+  (at level 99, E1,E2, k at level 50, Q at level 200,
+   format "'[' P  '/' = k ={ E1 , E2 }=∗  Q ']'").
+
+Notation "| k ={ E1 , E2 }=> Q" := (uPred_fupd_level E1 E2 k Q) : bi_scope.
+Notation "| k ={ E1 }=> Q" := (uPred_fupd_level E1 E1 k Q) : bi_scope.
+Notation "P = k ={ E1 , E2 }=∗ Q" := (P -∗ |k={E1,E2}=> Q)%I : bi_scope.
+Notation "P = k ={ E1 , E2 }=∗ Q" := (P -∗ |k={E1,E2}=> Q) : stdpp_scope.
+
+Section fupd_level.
+Context `{!invG Σ}.
+Implicit Types P: iProp Σ.
+Implicit Types E : coPset.
+Implicit Types k : nat.
+
+Global Instance fupd_level_ne E1 E2 k: NonExpansive (uPred_fupd_level E1 E2 k).
+Proof. rewrite uPred_fupd_level_eq. solve_proper. Qed.
+
+Lemma fupd_level_intro_mask E1 E2 k P : E2 ⊆ E1 → P ⊢ |k={E1,E2}=> |k={E2,E1}=> P.
+Proof.
+  intros (E1''&->&?)%subseteq_disjoint_union_L.
+  rewrite uPred_fupd_level_eq /uPred_fupd_level_def ownE_op //.
+  by iIntros "$ ($ & $ & HE) !> !> [$ $] !> !>" .
+Qed.
+
+Lemma except_0_fupd_level E1 E2 k P : ◇ (|k={E1,E2}=> P) ⊢ |k={E1,E2}=> P.
+Proof.
+  rewrite uPred_fupd_level_eq /uPred_fupd_level_def.
+  iIntros ">H [Hw HE]". iApply "H"; by iFrame.
+Qed.
+
+Lemma fupd_level_mono E1 E2 k P Q : (P ⊢ Q) → (|k={E1,E2}=> P) ⊢ |k={E1,E2}=> Q.
+Proof.
+  rewrite uPred_fupd_level_eq. iIntros (HPQ) "HP HwE". rewrite -HPQ. by iApply "HP".
+Qed.
+
+Lemma fupd_level_le E1 E2 k1 k2 P : k1 ≤ k2 → (|k1={E1,E2}=> P) ⊢ |k2={E1,E2}=> P.
+Proof.
+  rewrite ?uPred_fupd_level_eq /uPred_fupd_level_def.
+  iIntros (Hle) "HP (Hw&HE)".
+  iDestruct (wsat_le_acc (S k1) (S k2) with "Hw") as "(Hw&Hclo)".
+  { lia. }
+  iMod ("HP" with "[$]") as "H". iModIntro.
+  iMod "H" as "(Hw&HE)". iFrame.
+  iModIntro. by iApply "Hclo".
+Qed.
+
+Lemma fupd_level_fupd E1 E2 P k : (|k={E1,E2}=> P) ⊢ |={E1,E2}=> P.
+Proof.
+  rewrite ?uPred_fupd_level_eq /uPred_fupd_level_def.
+  rewrite ?uPred_fupd_eq /uPred_fupd_def.
+  iIntros "HP (Hw&HE)". iMod (wsat_all_acc (S k) with "Hw") as "(Hw&Hclo)".
+  iMod ("HP" with "[$]") as ">(?&$&$)".
+  do 2 iModIntro. by iApply "Hclo".
+Qed.
+
+Lemma fupd_level_trans E1 E2 E3 k P : (|k={E1,E2}=> |k={E2,E3}=> P) ⊢ |k={E1,E3}=> P.
+Proof.
+  rewrite uPred_fupd_level_eq. iIntros "HP HwE".
+  iMod ("HP" with "HwE") as ">(Hw & HE & HP)". iApply "HP"; by iFrame.
+Qed.
+
+Lemma fupd_level_mask_frame_r' E1 E2 Ef k P:
+    E1 ## Ef → (|k={E1,E2}=> ⌜E2 ## Ef⌝ → P) ⊢ |k={E1 ∪ Ef,E2 ∪ Ef}=> P.
+Proof.
+  intros HE1Ef. rewrite uPred_fupd_level_eq /uPred_fupd_level_def ownE_op //.
+  iIntros "Hvs (Hw & HE1 &HEf)".
+  iMod ("Hvs" with "[Hw HE1]") as ">($ & HE2 & HP)"; first by iFrame.
+  iDestruct (ownE_op' with "[HE2 HEf]") as "[? $]"; first by iFrame.
+  iIntros "!> !>". by iApply "HP".
+Qed.
+
+Lemma fupd_level_frame_r E1 E2 k P R:
+  (|k={E1,E2}=> P) ∗ R ⊢ |k={E1,E2}=> P ∗ R.
+Proof.
+  rewrite uPred_fupd_level_eq /uPred_fupd_level_def. by iIntros "[HwP $]".
+Qed.
+
+(*
+Instance uPred_bi_fupd_level `{!invG Σ} : BiFUpd (uPredI (iResUR Σ)) :=
+  {| bi_fupd_mixin := uPred_fupd_level_mixin |}.
+
+Instance uPred_bi_bupd_fupd_level `{!invG Σ} : BiBUpdFUpd (uPredI (iResUR Σ)).
+Proof. rewrite /BiBUpdFupd_Level uPred_fupd_level_eq. by iIntros (E P) ">? [$ $] !> !>". Qed.
+*)
+
+(*
+Instance uPred_bi_fupd_level_plainly `{!invG Σ} : BiFUpdPlainly (uPredI (iResUR Σ)).
+Proof.
+  split.
+  - rewrite uPred_fupd_level_eq /uPred_fupd_level_def. iIntros (E P) "H [Hw HE]".
+    iAssert (◇ ■ P)%I as "#>HP".
+    { by iMod ("H" with "[$]") as "(_ & _ & HP)". }
+    by iFrame.
+  - rewrite uPred_fupd_level_eq /uPred_fupd_level_def. iIntros (E P Q) "[H HQ] [Hw HE]".
+    iAssert (◇ ■ P)%I as "#>HP".
+    { by iMod ("H" with "HQ [$]") as "(_ & _ & HP)". }
+    by iFrame.
+  - rewrite uPred_fupd_level_eq /uPred_fupd_level_def. iIntros (E P) "H [Hw HE]".
+    iAssert (▷ ◇ ■ P)%I as "#HP".
+    { iNext. by iMod ("H" with "[$]") as "(_ & _ & HP)". }
+    iFrame. iIntros "!> !> !>". by iMod "HP".
+  - rewrite uPred_fupd_level_eq /uPred_fupd_level_def. iIntros (E A Φ) "HΦ [Hw HE]".
+    iAssert (◇ ■ ∀ x : A, Φ x)%I as "#>HP".
+    { iIntros (x). by iMod ("HΦ" with "[$Hw $HE]") as "(_&_&?)". }
+    by iFrame.
+Qed.
+*)
+Global Instance fupd_level_proper E1 E2 k :
+  Proper ((≡) ==> (≡)) (uPred_fupd_level E1 E2 k) := ne_proper _.
+
+Global Instance fupd_mono' E1 E2 k : Proper ((⊢) ==> (⊢)) (uPred_fupd_level E1 E2 k).
+Proof. intros P Q; apply fupd_level_mono. Qed.
+Global Instance fupd_flip_mono' E1 E2 k :
+  Proper (flip (⊢) ==> flip (⊢)) (uPred_fupd_level E1 E2 k).
+Proof. intros P Q; apply fupd_level_mono. Qed.
+
+Lemma bupd_fupd_level E k P:
+  (|==> P) ⊢ |k={E}=> P.
+Proof. rewrite uPred_fupd_level_eq. by iIntros ">? [$ $] !> !>". Qed.
+
+Lemma fupd_level_intro E k P : P ⊢ |k={E}=> P.
+Proof. by rewrite {1}(fupd_level_intro_mask E E k P) // fupd_level_trans. Qed.
+Lemma fupd_level_intro_mask' E1 E2 k : E2 ⊆ E1 → ⊢@{iPropI Σ} |k={E1,E2}=> |k={E2,E1}=> emp.
+Proof. exact: fupd_level_intro_mask. Qed.
+Lemma fupd_level_except_0 E1 E2 k P : (|k={E1,E2}=> ◇ P) ⊢ |k={E1,E2}=> P.
+Proof. by rewrite {1}(fupd_level_intro E2 k P) except_0_fupd_level fupd_level_trans. Qed.
+
+Global Instance from_assumption_fupd_level E k p P Q :
+  FromAssumption p P (|==> Q) → KnownRFromAssumption p P (|k={E}=> Q)%I.
+Proof. rewrite /KnownRFromAssumption /FromAssumption=>->. apply bupd_fupd_level. Qed.
+
+Global Instance from_pure_fupd_level a E k P φ :
+  FromPure a P φ → FromPure a (|k={E}=> P) φ.
+Proof. rewrite /FromPure. intros <-. apply fupd_level_intro. Qed.
+
+Lemma fupd_level_frame_l E1 E2 k R Q : (R ∗ |k={E1,E2}=> Q) ⊢ |k={E1,E2}=> R ∗ Q.
+Proof. rewrite !(comm _ R); apply fupd_level_frame_r. Qed.
+Lemma fupd_level_wand_l E1 E2 k P Q : (P -∗ Q) ∗ (|k={E1,E2}=> P) ⊢ |k={E1,E2}=> Q.
+Proof. by rewrite fupd_level_frame_l wand_elim_l. Qed.
+Lemma fupd_level_wand_r E1 E2 k P Q : (|k={E1,E2}=> P) ∗ (P -∗ Q) ⊢ |k={E1,E2}=> Q.
+Proof. by rewrite fupd_level_frame_r wand_elim_r. Qed.
+
+Lemma fupd_level_mask_weaken E1 E2 k P : E2 ⊆ E1 → P ⊢ |k={E1,E2}=> P.
+Proof.
+  intros ?. rewrite -{1}(right_id emp%I bi_sep P%I).
+  rewrite (fupd_level_intro_mask E1 E2 k emp%I) //.
+  by rewrite fupd_level_frame_l sep_elim_l.
+Qed.
+
+Lemma fupd_level_mask_frame_r E1 E2 k Ef P :
+  E1 ## Ef → (|k={E1,E2}=> P) ⊢ |k={E1 ∪ Ef,E2 ∪ Ef}=> P.
+Proof.
+  intros ?. rewrite -fupd_level_mask_frame_r' //. f_equiv.
+  apply impl_intro_l, and_elim_r.
+Qed.
+Lemma fupd_level_mask_mono E1 E2 k P : E1 ⊆ E2 → (|k={E1}=> P) ⊢ |k={E2}=> P.
+Proof.
+  intros (Ef&->&?)%subseteq_disjoint_union_L. by apply fupd_level_mask_frame_r.
+Qed.
+
+Lemma fupd_level_sep E k P Q : (|k={E}=> P) ∗ (|k={E}=> Q) ⊢ |k={E}=> P ∗ Q.
+Proof. by rewrite fupd_level_frame_r fupd_level_frame_l fupd_level_trans. Qed.
+Lemma fupd_level_mask_frame E E' E1 E2 k P :
+  E1 ⊆ E →
+  (|k={E1,E2}=> |k={E2 ∪ (E ∖ E1),E'}=> P) -∗ (|k={E,E'}=> P).
+Proof.
+  intros ?. rewrite (fupd_level_mask_frame_r _ _ _ (E ∖ E1)); last set_solver.
+  rewrite fupd_level_trans.
+  by replace (E1 ∪ E ∖ E1) with E by (by apply union_difference_L).
+Qed.
+
+Global Instance into_wand_fupd_level E k p q R P Q :
+  IntoWand false false R P Q →
+  IntoWand p q (|k={E}=> R) (|k={E}=> P) (|k={E}=> Q).
+Proof.
+  rewrite /IntoWand /= => HR. rewrite !intuitionistically_if_elim HR.
+  apply wand_intro_l. by rewrite fupd_level_sep wand_elim_r.
+Qed.
+
+Global Instance into_wand_fupd_level_persistent E1 E2 k p q R P Q :
+  IntoWand false q R P Q → IntoWand p q (|k={E1,E2}=> R) P (|k={E1,E2}=> Q).
+Proof.
+  rewrite /IntoWand /= => HR. rewrite intuitionistically_if_elim HR.
+  apply wand_intro_l. by rewrite fupd_level_frame_l wand_elim_r.
+Qed.
+
+Global Instance into_wand_fupd_level_args E1 E2 k p q R P Q :
+  IntoWand p false R P Q → IntoWand' p q R (|k={E1,E2}=> P) (|k={E1,E2}=> Q).
+Proof.
+  rewrite /IntoWand' /IntoWand /= => ->.
+  apply wand_intro_l. by rewrite intuitionistically_if_elim fupd_level_wand_r.
+Qed.
+
+Global Instance from_sep_fupd_level E k P Q1 Q2 :
+  FromSep P Q1 Q2 → FromSep (|k={E}=> P) (|k={E}=> Q1) (|k={E}=> Q2).
+Proof. rewrite /FromSep =><-. apply fupd_level_sep. Qed.
+
+Global Instance from_or_fupd_level E1 E2 k P Q1 Q2 :
+  FromOr P Q1 Q2 → FromOr (|k={E1,E2}=> P) (|k={E1,E2}=> Q1) (|k={E1,E2}=> Q2).
+  rewrite /FromOr=><-. apply or_elim; apply fupd_level_mono;
+                         [apply bi.or_intro_l|apply bi.or_intro_r].
+Qed.
+
+Global Instance from_exist_fupd_level {A} E1 k E2 P (Φ : A → iProp Σ) :
+  FromExist P Φ → FromExist (|k={E1,E2}=> P) (λ a, |k={E1,E2}=> Φ a)%I.
+Proof.
+  rewrite /FromExist=><-. apply exist_elim=> a. by rewrite -(exist_intro a).
+Qed.
+
+(*
+Global Instance from_forall_fupd_level E1 E2 k {A} P (Φ : A → iProp Σ) :
+  (* Some cases in which [E2 ⊆ E1] holds *)
+  TCOr (TCEq E1 E2) (TCOr (TCEq E1 ⊤) (TCEq E2 ∅)) →
+  FromForall P Φ → (∀ x, Plain (Φ x)) →
+  FromForall (|k={E1,E2}=> P)%I (λ a, |k={E1,E2}=> (Φ a))%I.
+Proof.
+  rewrite /FromForall=> -[->|[->|->]] <- ?; rewrite fupd_plain_forall; set_solver.
+Qed.
+*)
+
+Global Instance except_0_fupd_level' E1 E2 k P :
+  IsExcept0 (|k={E1,E2}=> P).
+Proof. by rewrite /IsExcept0 except_0_fupd_level. Qed.
+
+Global Instance from_modal_fupd_level E k P :
+  FromModal modality_id (|k={E}=> P) (|k={E}=> P) P.
+Proof. by rewrite /FromModal /= -fupd_level_intro. Qed.
+
+Global Instance elim_modal_bupd_fupd_level p E1 E2 k P Q :
+  ElimModal True p false (|==> P) P (|k={E1,E2}=> Q) (|k={E1,E2}=> Q) | 10.
+Proof.
+   by rewrite /ElimModal intuitionistically_if_elim
+    (bupd_fupd_level E1 k) fupd_level_frame_r wand_elim_r fupd_level_trans.
+Qed.
+Global Instance elim_modal_fupd_level_fupd_level p E1 E2 E3 k P Q :
+  ElimModal True p false (|k={E1,E2}=> P) P (|k={E1,E3}=> Q) (|k={E2,E3}=> Q).
+Proof.
+  by rewrite /ElimModal intuitionistically_if_elim
+    fupd_level_frame_r wand_elim_r fupd_level_trans.
+Qed.
+(*
+Global Instance elim_modal_fupd_fupd_level p E1 E2 k P Q :
+  ElimModal True p false (|={E1,E2}=> P) P (|(S k)={E1,E3}=> Q) (|(S k)={E2,E3}=> Q).
+Proof.
+  rewrite /ElimModal => ??. rewrite (fupd_fupd_level _ _ k) intuitionistically_if_elim
+    fupd_level_frame_r wand_elim_r fupd_level_trans //=.
+Qed.
+*)
+
+Global Instance elim_acc_fupd_level {X} E1 E2 E k α β mγ Q :
+  ElimAcc (X:=X) (uPred_fupd_level E1 E2 k) (uPred_fupd_level E2 E1 k) α β mγ
+          (|k={E1,E}=> Q)
+          (λ x, |k={E2}=> β x ∗ (mγ x -∗? |k={E1,E}=> Q))%I.
+Proof.
+  rewrite /ElimAcc.
+  iIntros "Hinner >Hacc". iDestruct "Hacc" as (x) "[Hα Hclose]".
+  iMod ("Hinner" with "Hα") as "[Hβ Hfin]".
+  iMod ("Hclose" with "Hβ") as "Hγ". by iApply "Hfin".
+Qed.
+
+Global Instance frame_fupd_level p E1 E2 k R P Q :
+  Frame p R P Q → Frame p R (|k={E1,E2}=> P) (|k={E1,E2}=> Q).
+Proof. rewrite /Frame=><-. by rewrite fupd_level_frame_l. Qed.
+
+Lemma fupd_level_mask_mono' E1 E2 E1' E2' k P : E1 ⊆ E2 → E2' ⊆ E1' → (|k={E1, E1'}=> P) ⊢ |k={E2,E2'}=> P.
+Proof.
+  iIntros (??) "H".
+  iMod (fupd_level_intro_mask' _ E1) as "Hclo"; auto.
+  iMod "H".
+  iApply (fupd_level_mask_weaken); auto.
+Qed.
+
+Lemma step_fupd_level_mask_mono Eo1 Eo2 Ei1 Ei2 k P :
+  Ei2 ⊆ Ei1 → Eo1 ⊆ Eo2 →
+  (|k={Eo1,Ei1}=> ▷ |k={Ei1, Eo1}=> P) ⊢ (|k={Eo2,Ei2}=> ▷ |k={Ei2, Eo2}=> P).
+Proof.
+  intros ??. rewrite -(emp_sep (|k={Eo1,Ei1}=> ▷ _))%I.
+  rewrite (fupd_level_intro_mask Eo2 Eo1 _ emp%I) //.
+  rewrite fupd_level_frame_r -(fupd_level_trans Eo2 Eo1 Ei2). f_equiv.
+  rewrite fupd_level_frame_l -(fupd_level_trans Eo1 Ei1 Ei2). f_equiv.
+  rewrite (fupd_level_intro_mask Ei1 Ei2 _ (|k={_,_}=> emp)%I) //.
+  rewrite fupd_level_frame_r. f_equiv.
+  rewrite [X in (X ∗ _)%I]later_intro -later_sep. f_equiv.
+  rewrite fupd_level_frame_r -(fupd_level_trans Ei2 Ei1 Eo2). f_equiv.
+  rewrite fupd_level_frame_l -(fupd_level_trans Ei1 Eo1 Eo2). f_equiv.
+  by rewrite fupd_level_frame_r left_id.
+Qed.
+
+Lemma step_fupd_level_intro Ei Eo k P : Ei ⊆ Eo → ▷ P -∗ |k={Eo,Ei}=> ▷ |k={Ei,Eo}=> P.
+Proof. intros. by rewrite -(step_fupd_level_mask_mono Ei _ Ei _) // -!fupd_level_intro. Qed.
+
+End fupd_level.
+
+Section fupd_level.
+Context `{!invG Σ}.
+Implicit Types P: iProp Σ.
+Implicit Types E : coPset.
+Implicit Types k : nat.
+
+Lemma fupd_level_plain_soundness `{!invPreG Σ} E1 E2 k (P: iProp Σ) `{!Plain P} :
+  (∀ `{Hinv: !invG Σ}, ⊢ |k={E1,E2}=> P) → ⊢ P.
+Proof.
+  iIntros (Hfupd_level). apply (later_soundness _); simpl.
+   iMod wsat_alloc as (Hinv) "[Hw HE]".
+  iAssert (|k={⊤,E2}=> P)%I as "H".
+  { iMod (fupd_level_intro_mask'); last iApply Hfupd_level. done. }
+  rewrite uPred_fupd_level_eq /uPred_fupd_level_def.
+  iMod ("H" with "[$]") as "[Hw [HE >H']]"; iFrame.
+Qed.
+
+(*
+Lemma step_fupd_levelN_soundness `{!invPreG Σ} φ n :
+  (∀ `{Hinv: !invG Σ}, ⊢@{iPropI Σ} |={⊤}[∅]▷=>^n |={⊤,∅}=> ⌜ φ ⌝) →
+  φ.
+Proof.
+  intros Hiter.
+  apply (soundness (M:=iResUR Σ) _  (S n)); simpl.
+  apply (fupd_level_plain_soundness ⊤ ⊤ _)=> Hinv.
+  iPoseProof (Hiter Hinv) as "H". clear Hiter.
+  destruct n as [|n].
+  - iApply fupd_level_plainly_mask_empty. iMod "H" as %?; auto.
+  - iDestruct (step_fupd_levelN_wand _ _ _ _ (|={⊤}=> ⌜φ⌝)%I with "H []") as "H'".
+    { by iApply fupd_level_plain_mask_empty. }
+    rewrite -step_fupd_levelN_S_fupd_level.
+    iMod (step_fupd_levelN_plain with "H'") as "Hφ". iModIntro. iNext.
+    rewrite -later_laterN laterN_later.
+    iNext. by iMod "Hφ".
+Qed.
+
+Lemma step_fupd_levelN_soundness' `{!invPreG Σ} φ n :
+  (∀ `{Hinv: !invG Σ}, ⊢@{iPropI Σ} |={⊤}[∅]▷=>^n ⌜ φ ⌝) →
+  φ.
+Proof.
+  iIntros (Hiter). eapply (step_fupd_levelN_soundness _ n).
+  iIntros (Hinv). iPoseProof (Hiter Hinv) as "Hiter".
+  iApply (step_fupd_levelN_wand with "Hiter"). by iApply fupd_level_mask_weaken.
+Qed.
+ *)
+End fupd_level.
